Fir/Wasm/Concrete.lean
@@ -9,3 +9,4 @@ import Fir.Wasm.Concrete.ObjectFieldsCorrectness
 import Fir.Wasm.Concrete.FreshAllocationCorrectness
 import Fir.Wasm.Concrete.HeapRefinement
 import Fir.Wasm.Concrete.ConstructorAllocationCorrectness
+import Fir.Wasm.Concrete.ConstructorHeapCorrectness
